src/goose_lang/lib/slice/typed_slice.v
@@ -194,8 +194,8 @@ Proof.
   rewrite /is_slice_small /list.untype list_fmap_insert. iFrame.
 Qed.
 
-Lemma wp_SliceAppend'' stk E s t `{!IntoValForType IntoVal0 t} vs1 vs2 (x: V) (q : Qp) n :
-  0 ≤ n ≤ int.val (Slice.sz s) ≤ int.val (Slice.cap s) ->
+Lemma wp_SliceAppend'' stk E s t `{!IntoValForType IntoVal0 t} vs1 vs2 (x: V) (q : Qp) (n : u64) :
+  0 ≤ int.val n ≤ int.val (Slice.sz s) ≤ int.val (Slice.cap s) ->
   (Qcanon.Qclt q 1)%Qc ->
   {{{ is_slice_small (slice_take s t n) t q vs1 ∗
       is_slice (slice_skip s t n) t 1 vs2 }}}
@@ -203,7 +203,8 @@ Lemma wp_SliceAppend'' stk E s t `{!IntoValForType IntoVal0 t} vs1 vs2 (x: V) (q
   {{{ s', RET slice_val s';
       is_slice_small (slice_take s' t n) t q vs1 ∗
       is_slice (slice_skip s' t n) t 1 (vs2 ++ [x]) ∗
-      ⌜int.val (Slice.sz s') ≤ int.val (Slice.cap s')⌝}}}.
+      ⌜int.val (Slice.sz s') ≤ int.val (Slice.cap s') ∧
+       int.val (Slice.sz s') = (int.val (Slice.sz s) + 1)%Z⌝}}}.
 Proof.
   iIntros (Hn Hq Φ) "[Hsm Hs] HΦ".
   wp_apply (slice.wp_SliceAppend'' with "[$Hsm $Hs]").
